Regex/Regex.lean
@@ -2,6 +2,7 @@ inductive Regex : Type where
   | empty : Regex
   | epsilon : Regex
   | char : Char → Regex
+  | group : Nat → Regex → Regex
   | alternate : Regex → Regex → Regex
   | concat : Regex → Regex → Regex
   | star : Regex → Regex
@@ -10,6 +11,7 @@ deriving Repr, Inhabited
 inductive Regex.matches : String → Regex → Prop where
   | char (c : Char) (eq : s = ⟨[c]⟩): Regex.matches s (.char c)
   | epsilon (eq : s = "") : Regex.matches s .epsilon
+  | group (m : Regex.matches s r) : Regex.matches s (.group i r)
   | alternateLeft {s : String} {r₁ r₂ : Regex} : Regex.matches s r₁ → Regex.matches s (.alternate r₁ r₂)
   | alternateRight {s : String} {r₁ r₂ : Regex} : Regex.matches s r₂ → Regex.matches s (.alternate r₁ r₂)
   | concat (s s₁ s₂ : String) (r₁ r₂ : Regex) (eq : s = s₁ ++ s₂) :
@@ -30,15 +32,17 @@ theorem Regex.char_matches (m : Regex.matches s (.char c)) : s = ⟨[c]⟩ :=
   match s, m with
   | _, .char _ eq => eq
 
+theorem Regex.group_matches : Regex.matches s (.group i r) ↔ Regex.matches s r :=
+  ⟨fun | .group m => m, .group⟩
+
 theorem Regex.alternate_matches_or : Regex.matches s (.alternate r₁ r₂) ↔ Regex.matches s r₁ ∨ Regex.matches s r₂ :=
-  ⟨fun m => match s, m with
-    | _, .alternateLeft m => Or.inl m
-    | _, .alternateRight m => Or.inr m,
+  ⟨fun
+    | .alternateLeft m => Or.inl m
+    | .alternateRight m => Or.inr m,
    fun
     | Or.inl m => .alternateLeft m
     | Or.inr m => .alternateRight m⟩
 
 theorem Regex.concat_matches : Regex.matches s (.concat r₁ r₂) ↔ ∃s₁ s₂, s = s₁ ++ s₂ ∧ Regex.matches s₁ r₁ ∧ Regex.matches s₂ r₂ :=
-  ⟨fun m => match s, m with
-    | _, .concat _ _ _ _ _ eq m₁ m₂ => ⟨_, _, eq, m₁, m₂⟩,
+  ⟨fun | .concat _ _ _ _ _ eq m₁ m₂ => ⟨_, _, eq, m₁, m₂⟩,
    fun ⟨s₁, s₂, eq, m₁, m₂⟩ => .concat s s₁ s₂ r₁ r₂ eq m₁ m₂⟩
