Regex/Parser/Hir.lean
@@ -1,0 +1,37 @@
+import Regex.Regex
+
+namespace Regex.Parser
+
+inductive Hir : Type where
+  | empty : Hir
+  | epsilon : Hir
+  | char : Char → Hir
+  | group : Hir → Hir
+  | alternate : Hir → Hir → Hir
+  | concat : Hir → Hir → Hir
+  | star : Hir → Hir
+deriving Repr, Inhabited
+
+def Hir.toRegexAux (index : Nat) (hir : Hir) : Nat × Regex :=
+  match hir with
+  | .empty => (index, .empty)
+  | .epsilon => (index, .epsilon)
+  | .char c => (index, .char c)
+  | .group h =>
+    let (index', r) := h.toRegexAux (index + 1)
+    (index', .group index r)
+  | .alternate h₁ h₂ =>
+    let (index₁, r₁) := h₁.toRegexAux index
+    let (index₂, r₂) := h₂.toRegexAux index₁
+    (index₂, .alternate r₁ r₂)
+  | .concat h₁ h₂ =>
+    let (index₁, r₁) := h₁.toRegexAux index
+    let (index₂, r₂) := h₂.toRegexAux index₁
+    (index₂, .concat r₁ r₂)
+  | .star h =>
+    let (index', r) := h.toRegexAux index
+    (index', .star r)
+
+def Hir.toRegex (h : Hir) : Regex := (h.toRegexAux 0).2
+
+end Regex.Parser
